tuned

Primitive_Matchers/Primitive_Abstract.thy
@@ -26,7 +26,9 @@ fun abstract_primitive :: "(common_primitive negation_type \<Rightarrow> bool) \
 text{*For example, a simple firewall requires that no negated interfaces and protocols occur in the 
       expression. *}
 definition abstract_for_simple_firewall :: "common_primitive match_expr \<Rightarrow> common_primitive match_expr"
-  where "abstract_for_simple_firewall \<equiv> abstract_primitive (\<lambda>r. case r of Pos a \<Rightarrow> is_CT_State a | Neg a \<Rightarrow> is_Iiface a \<or> is_Oiface a \<or> is_Prot a \<or> is_CT_State a)"
+  where "abstract_for_simple_firewall \<equiv> abstract_primitive (\<lambda>r. case r
+                of Pos a \<Rightarrow> is_CT_State a \<or> is_L4_Flags a
+                |  Neg a \<Rightarrow> is_Iiface a \<or> is_Oiface a \<or> is_Prot a \<or> is_CT_State a \<or> is_L4_Flags a)"
 
 
 text{*The function @{const ctstate_assume_state} can be used to fix a state and hence remove all state matches from the ruleset.
@@ -34,6 +36,17 @@ text{*The function @{const ctstate_assume_state} can be used to fix a state and 
       calling to @{const abstract_for_simple_firewall}.*}
 lemma not_hasdisc_ctstate_assume_state: "\<not> has_disc is_CT_State (ctstate_assume_state s m)"
   by(induction m rule: ctstate_assume_state.induct) (simp_all)
+
+
+lemma abstract_for_simple_firewall_hasdisc:
+  "\<not> has_disc is_CT_State (abstract_for_simple_firewall m)"
+  "\<not> has_disc is_L4_Flags (abstract_for_simple_firewall m)"
+  unfolding abstract_for_simple_firewall_def
+  apply(induction "(\<lambda>r. case r of Pos a \<Rightarrow> is_CT_State a | Neg a \<Rightarrow> is_Iiface a \<or> is_Oiface a \<or> is_Prot a \<or> is_CT_State a)" m rule: abstract_primitive.induct)
+  apply(simp_all)
+  done
+  
+
 
 context
 begin
